finishes impl. of quantified signatures

theories/logic/sem_sig.v
@@ -21,59 +21,60 @@ Lemma sem_sig_to_ieff {Σ} (σ σ' : sem_sig Σ) :
     σ ≤S σ' -∗ iEff_le σ σ'.
 Proof. iIntros "H". rewrite /sig_le. iApply "H". Qed.
 
-(* Single Variable Universally Quantified Effect Signatures *)
+(* Universally Quantified Effect Signatures *)
+
 (* Effect Signature *)
-Definition sem_sig_eff {Σ} m (A B : sem_ty Σ -d> sem_ty Σ) : sem_sig Σ :=
-  (>> (α : sem_ty Σ) (a : val) >> ! a {{ ▷ (A α a) }}; 
-   << (b : val)                << ? b {{ ▷ (B α b) }} @m)%ieff.
+Definition sem_sig_eff {Σ} {TT : tele} m (A B : TT → sem_ty Σ) : sem_sig Σ :=
+  (>>.. (αs : TT) >> >> (a : val) >>  ! a {{ ▷ (A αs a) }}; 
+                     << (b : val) <<  ? b {{ ▷ (B αs b) }} @m)%ieff.
 
-Lemma sem_sig_eff_unfold {Σ} m (A B : sem_ty Σ -d> sem_ty Σ) :
-  (sem_sig_eff m A B) ≡
-    (>> (α : sem_ty Σ) (a : val) >> ! a {{ ▷ (A α a) }}; 
-     << (b : val)                << ? b {{ ▷ (B α b) }} @m)%ieff.
-Proof. by rewrite /sem_sig_eff. Qed.
+Lemma sem_sig_eff_unfold {Σ} {TT : tele} m (A B : TT → sem_ty Σ) :
+  (sem_sig_eff m A B) ≡ 
+  (>>.. (αs : TT) >> >> (a : val) >> ! a {{ ▷ (A αs a) }}; 
+                     << (b : val) << ? b {{ ▷ (B αs b) }} @m)%ieff.
+Proof. rewrite /sem_sig_eff //. Qed.
 
-Lemma sem_sig_eff_unfold_iEff {Σ} m (A B : sem_ty Σ -d> sem_ty Σ) v Φ:
+Lemma sem_sig_eff_unfold_iEff {Σ} {TT : tele} m (A B : TT → sem_ty Σ) v Φ:
   iEff_car (sem_sig_eff m A B) v Φ ⊣⊢
-    iEff_car (>> (α : sem_ty Σ) (a : val) >> ! a {{ ▷ (A α a) }}; 
-              << (b : val)                << ? b {{ ▷ (B α b) }} @m)%ieff v Φ.
+    iEff_car (>>.. (αs : TT) >> >> (a : val) >> ! a {{ ▷ (A αs a) }}; 
+                                << (b : val) << ? b {{ ▷ (B αs b) }} @m)%ieff v Φ.
 Proof. done. Qed.
 
-Lemma sem_sig_eff_eq {Σ} m A B v Φ :
-  iEff_car (@sem_sig_eff Σ m A B) v Φ ⊣⊢
-    (∃ α a, ⌜ a = v ⌝ ∗ ▷ (A α a) ∗ 
-                        □? m (∀ b, ▷ (B α b) -∗ Φ b))%I.
+Lemma sem_sig_eff_eq {Σ} {TT : tele} m A B v Φ :
+  iEff_car (@sem_sig_eff Σ TT m A B) v Φ ⊣⊢
+    (∃.. αs, ∃ a, ⌜ a = v ⌝ ∗ ▷ (A αs a) ∗ 
+                             □? m (∀ b, ▷ (B αs b) -∗ Φ b))%I.
 Proof. 
-  etrans; [by apply sem_sig_eff_unfold_iEff|]. 
-  by rewrite (iEff_tele_eq' [tele _ _] [tele _]) /=. 
+  rewrite iEffPre_texist_eq. do 2 f_equiv.
+  rewrite (iEff_tele_eq' [tele _] [tele _]) //. 
 Qed.
 
 (* The sem_sig_eff protocol is monotonic. *)
-Global Instance sem_sig_eff_mono_prot {Σ} A B :
-  MonoProt (@sem_sig_eff Σ OS A B).
+Global Instance sem_sig_eff_mono_prot {Σ} {TT : tele} A B :
+  MonoProt (@sem_sig_eff Σ TT OS A B).
 Proof.
   constructor. iIntros (???) "HΦ'".
   rewrite !sem_sig_eff_eq /=.
   iIntros "(% & % & <- & Hτ & HκΦ)".
-  iExists α, a. iSplitR; first done. iFrame. simpl.
+  iExists αs, a. iSplitR; first done. iFrame. simpl.
   iIntros (b) "Hκ". iApply "HΦ'". by iApply "HκΦ".
 Qed.
 
 (* The sem_sig_eff protocol is persistently monotonic. *)
-Global Instance sem_sig_eff_pers_mono_prot {Σ} A B :
-  PersMonoProt (@sem_sig_eff Σ MS A B).
+Global Instance sem_sig_eff_pers_mono_prot {Σ} {TT : tele} A B :
+  PersMonoProt (@sem_sig_eff Σ TT MS A B).
 Proof.
   constructor. iIntros (???) "#HΦ'".
   rewrite !sem_sig_eff_eq. simpl.
   iIntros "(% & % & <- & Hτ & #HκΦ)".
-  iExists α, a. iSplitR; first done. iFrame. simpl.
+  iExists αs, a. iSplitR; first done. iFrame. simpl.
   iIntros "!# %b Hκ". iApply "HΦ'". by iApply "HκΦ".
 Qed.
 
-Lemma upcl_sem_sig_eff {Σ} m A B v Φ :
-  iEff_car (upcl m (@sem_sig_eff Σ m A B)) v Φ ⊣⊢
-    (∃ α a, ⌜ a = v ⌝ ∗ ▷ (A α a) ∗ 
-                        □? m (∀ b, ▷ (B α b) -∗ Φ b))%I.
+Lemma upcl_sem_sig_eff {Σ} {TT : tele} m A B v Φ :
+  iEff_car (upcl m (@sem_sig_eff Σ TT m A B)) v Φ ⊣⊢
+    (∃.. αs, ∃ a, ⌜ a = v ⌝ ∗ ▷ (A αs a) ∗ 
+                              □? m (∀ b, ▷ (B αs b) -∗ Φ b))%I.
 Proof.
   assert (Hequiv:
     iEff_car (upcl m (sem_sig_eff m A B)) v Φ ≡ iEff_car (sem_sig_eff m A B) v Φ).
@@ -82,83 +83,17 @@ Proof.
 Qed.
 
 (* Notations. *)
-Notation "'∀S:' α , τ ⇒ κ | m " := (sem_sig_eff m (λ α, τ%T) (λ α, κ%T))
-  (at level 100, m, τ, κ at level 200) : sem_sig_scope.
+Notation "'∀S..:' tt , κ ⇒ ι | m" := 
+  (sem_sig_eff m (λ tt, κ%T) (λ tt, ι%T))
+  (at level 200, tt binder, right associativity,
+   format "'[ ' '∀S..:' tt ,  κ  ⇒  ι  |  m ']'") : sem_sig_scope.
 
-(* Multiple Variable Universally Quantified Effect Signatures *)
-
-(* Effect Signature *)
-Definition sem_sig_prot {Σ} {TT : tele} m (A B : TT → sem_ty Σ) : sem_sig Σ :=
-  (>>.. (αs : TT) >> >> (a : val) >>  ! a {{ ▷ (A αs a) }}; 
-                     << (b : val) <<  ? b {{ ▷ (B αs b) }} @m)%ieff.
-
-Lemma sem_sig_prot_unfold {Σ} {TT : tele} m (A B : TT → sem_ty Σ) :
-  (sem_sig_prot m A B) ≡ 
-  (>>.. (αs : TT) >> >> (a : val) >> ! a {{ ▷ (A αs a) }}; 
-                     << (b : val) << ? b {{ ▷ (B αs b) }} @m)%ieff.
-Proof. rewrite /sem_sig_prot //. Qed.
-
-Lemma sem_sig_prot_unfold_iEff {Σ} {TT : tele} m (A B : TT → sem_ty Σ) v Φ:
-  iEff_car (sem_sig_prot m A B) v Φ ⊣⊢
-    iEff_car (>>.. (αs : TT) >> >> (a : val) >> ! a {{ ▷ (A αs a) }}; 
-                                << (b : val) << ? b {{ ▷ (B αs b) }} @m)%ieff v Φ.
-Proof. done. Qed.
-
-Lemma sem_sig_prot_eq {Σ} {TT : tele} m A B v Φ :
-  iEff_car (@sem_sig_prot Σ TT m A B) v Φ ⊣⊢
-    (∃.. αs, ∃ a, ⌜ a = v ⌝ ∗ ▷ (A αs a) ∗ 
-                             □? m (∀ b, ▷ (B αs b) -∗ Φ b))%I.
-Proof. 
-  rewrite iEffPre_texist_eq. do 2 f_equiv.
-  rewrite (iEff_tele_eq' [tele _] [tele _]) //. 
-Qed.
-
-(* The sem_sig_prot protocol is monotonic. *)
-Global Instance sem_sig_prot_mono_prot {Σ} {TT : tele} A B :
-  MonoProt (@sem_sig_prot Σ TT OS A B).
-Proof.
-  constructor. iIntros (???) "HΦ'".
-  rewrite !sem_sig_prot_eq /=.
-  iIntros "(% & % & <- & Hτ & HκΦ)".
-  iExists αs, a. iSplitR; first done. iFrame. simpl.
-  iIntros (b) "Hκ". iApply "HΦ'". by iApply "HκΦ".
-Qed.
-
-(* The sem_sig_eff protocol is persistently monotonic. *)
-Global Instance sem_sig_prot_pers_mono_prot {Σ} {TT : tele} A B :
-  PersMonoProt (@sem_sig_prot Σ TT MS A B).
-Proof.
-  constructor. iIntros (???) "#HΦ'".
-  rewrite !sem_sig_prot_eq. simpl.
-  iIntros "(% & % & <- & Hτ & #HκΦ)".
-  iExists αs, a. iSplitR; first done. iFrame. simpl.
-  iIntros "!# %b Hκ". iApply "HΦ'". by iApply "HκΦ".
-Qed.
-
-Lemma upcl_sem_sig_prot {Σ} {TT : tele} m A B v Φ :
-  iEff_car (upcl m (@sem_sig_prot Σ TT m A B)) v Φ ⊣⊢
-    (∃.. αs, ∃ a, ⌜ a = v ⌝ ∗ ▷ (A αs a) ∗ 
-                              □? m (∀ b, ▷ (B αs b) -∗ Φ b))%I.
-Proof.
-  assert (Hequiv:
-    iEff_car (upcl m (sem_sig_prot m A B)) v Φ ≡ iEff_car (sem_sig_prot m A B) v Φ).
-  { f_equiv. apply non_dep_fun_equiv. destruct m; [by rewrite upcl_id|by rewrite pers_upcl_id]. }
-  rewrite Hequiv. by apply sem_sig_prot_eq.
-Qed.
-
-(* Notations. *)
-Notation "'∀S.:' x .. y , κ ⇒ ι | m" := 
-  (sem_sig_prot m
+Notation "'∀S:' x .. y , κ ⇒ ι | m" := 
+  (sem_sig_eff m
   (@tele_app ((TeleS (λ x, .. (TeleS (λ y, TeleO)) ..))) (sem_ty _) (λ x, .. (λ y, κ%T) ..)) 
   (@tele_app ((TeleS (λ x, .. (TeleS (λ y, TeleO)) ..))) (sem_ty _) (λ x, .. (λ y, ι%T) ..))) 
   (at level 200, x binder, y binder, right associativity,
-   format "'[ ' '∀S.:' x .. y ']' , κ ⇒ ι | m") : sem_sig_scope.
-
-(* Notations. *)
-Notation "'∀S..:' tt , κ ⇒ ι | m" := 
-  (sem_sig_prot m (λ tt, κ%T) (λ tt, ι%T))
-  (at level 200, tt binder, right associativity,
-   format "'[ ' '∀S..:' tt , κ ⇒ ι | m ']'") : sem_sig_scope.
+   format "'[ ' '∀S:' x .. y ,  κ  ⇒  ι  |  m ']'") : sem_sig_scope.
 
 (* Eval cbn in (∀S.: (α : sem_ty Σ), (sem_ty_prod α α) ⇒ (sem_ty_cpy α) | OS)%S. *)
 
@@ -181,18 +116,11 @@ Proof. inv MonoProt0. constructor. iIntros (v Φ Φ') "HPost Hσ".
        iApply (monotonic_prot0 v Φ Φ' with "HPost Hσ"). 
 Qed.
   
-Global Instance sig_eff_os_os_sig {Σ}  (A B : sem_ty Σ → sem_ty Σ) :
-  OSSig (∀S: α, A α ⇒ B α | OS)%S.
+Global Instance sig_eff_os_os_sig {TT : tele} {Σ} (A B : tele_arg TT → sem_ty Σ) :
+  OSSig (∀S..: αs , A αs ⇒ B αs | OS)%S.
 Proof. 
   apply mono_prot_os_sig.
   by apply sem_sig_eff_mono_prot.
-Qed.
-  
-Global Instance sig_prot_os_os_sig {TT : tele} {Σ} (A B : tele → sem_ty Σ) :
-  OSSig (∀S.: αs, A αs ⇒ B αs | OS)%S.
-Proof. 
-  apply mono_prot_os_sig.
-  by apply sem_sig_prot_mono_prot.
 Qed.
   
 Global Instance sig_os_os_sig {Σ} (σ : sem_sig Σ) : OSSig (¡ σ)%S.
@@ -215,31 +143,7 @@ Proof.
   iApply iEff_le_trans; [iApply "Hp₁₂"|iApply "Hp₂₃"].
 Qed.
 
-Lemma sig_le_eff {Σ} m₁ m₂ (ι₁ ι₂ κ₁ κ₂ : sem_ty Σ → sem_ty Σ) :
-  m₁ ≤M m₂ -∗
-  □ (∀ α, (ι₁ α) ≤T (ι₂ α)) -∗
-  □ (∀ α, (κ₂ α) ≤T (κ₁ α)) -∗
-  (∀S: α , ι₁ α ⇒ κ₁ α | m₁) ≤S (∀S: α , ι₂ α ⇒ κ₂ α | m₂).
-Proof.
-  iIntros "#Hmle #Hι₁₂ #Hκ₂₁". 
-  iIntros (v Φ) "!#".
-  rewrite !sem_sig_eff_eq.
-  iIntros "(%α & %w & <- & Hι₁ & HκΦ₁)".
-  iExists α, w; iSplitR; first done.
-  iSplitL "Hι₁".
-  { iApply ("Hι₁₂" with "Hι₁"). }
-  simpl. destruct m₁, m₂; rewrite /mode_le; eauto; simpl.
-  - iIntros (b) "Hκ₂". iApply "HκΦ₁".
-    iApply ("Hκ₂₁" with "Hκ₂").
-  - iDestruct "Hmle" as "[%|%]"; discriminate.
-  - iIntros (b) "Hκ₂". iApply "HκΦ₁".
-    iApply ("Hκ₂₁" with "Hκ₂").
-  - iDestruct "HκΦ₁" as "#HκΦ₁".
-    iIntros "!# %b Hκ₂". iApply "HκΦ₁".
-    iApply ("Hκ₂₁" with "Hκ₂").
-Qed.
-
-Lemma sig_le_prot {Σ} {TT : tele} m₁ m₂ (ι₁ ι₂ κ₁ κ₂ : TT → sem_ty Σ) :
+Lemma sig_le_eff {Σ} {TT : tele} m₁ m₂ (ι₁ ι₂ κ₁ κ₂ : tele_arg TT → sem_ty Σ) :
   m₁ ≤M m₂ -∗
   □ (∀.. α, (ι₁ α) ≤T (ι₂ α)) -∗
   □ (∀.. α, (κ₂ α) ≤T (κ₁ α)) -∗
@@ -247,7 +151,7 @@ Lemma sig_le_prot {Σ} {TT : tele} m₁ m₂ (ι₁ ι₂ κ₁ κ₂ : TT → s
 Proof.
   iIntros "#Hmle #Hι₁₂ #Hκ₂₁". 
   iIntros (v Φ) "!#".
-  rewrite !sem_sig_prot_eq.
+  rewrite !sem_sig_eff_eq.
   iIntros "(%α & %w & <- & Hι₁ & HκΦ₁)".
   iExists α, w; iSplitR; first done.
   iSplitL "Hι₁".
