theories/case_studies/generator_iterator.v
@@ -48,7 +48,7 @@ Section typing.
 
   Context `{!heapGS Σ}.
 
-  Definition yield_sig (τ : sem_ty Σ) : operation * sem_sig Σ := ("yield", ∀S: _, τ ⇒ () | OS)%S.
+  Definition yield_sig (τ : sem_ty Σ) : operation * sem_sig Σ := ("yield", ∀S: (_ : sem_ty Σ), τ ⇒ () | OS)%S.
   Definition yield_ty τ := τ -{ (yield_sig τ ·: ⟨⟩) }-> ().
   Definition iter_ty τ := (∀R: θ, (τ -{ θ }-> ()) -{ θ }-∘ ())%T.
   Definition generator_ty τ := (() → Option τ)%T.
@@ -62,14 +62,14 @@ Section typing.
     iApply (sem_typed_let (Refᶜ cont_ty) _ _ _ []); simpl; solve_sidecond. 
     - iApply sem_typed_alloc_cpy.
       rewrite -(app_nil_r [("i", _)]).
-      iApply sem_typed_afun; solve_sidecond. simpl.
+      iApply sem_typed_afun; solve_sidecond. 
       iApply (sem_typed_app_os (yield_ty α) _ _ _ [("i", iter_ty α)]); solve_sidecond.
       + iApply sem_typed_sub_nil.
         iApply (sem_typed_RApp (λ ρ, ( α -{ ρ }-> ()) -{ ρ }-∘ ())); solve_sidecond.
         iApply sem_typed_var.
       + iApply sem_typed_frame. iApply sem_typed_sub_nil.
         iApply sem_typed_val. rewrite /yield /yield_ty. iApply sem_typed_closure; solve_sidecond.
-        simpl. iApply (sem_typed_perform_os () with "[]"). 
+        simpl. iApply (sem_typed_perform_os (TT:=[tele _]) [tele_arg ()] with "[]"). 
         iApply sem_typed_var'.
     - set Γ₁ :=[("cont", Refᶜ cont_ty)]; rewrite -(app_nil_r Γ₁). 
       iApply sem_typed_ufun; solve_sidecond. simpl.
